concurrency/scache/cache/Cache_Refines_SimpleCache.i.dfy
@@ -1,0 +1,247 @@
+include "SimpleCacheSM.i.dfy"
+include "CacheSM.i.dfy"
+include "../Constants.i.dfy"
+
+module DiskSSM_Refines_SimpleCachine
+  refines Refinement(CrashAsyncIfc(CacheIfc),
+        AsyncDiskSystemStateMachine(CacheIfc, CacheSSM),
+        SimpleCacheStateMachine)
+{
+  import opened Constants
+  import opened RequestIds
+  import opened Options
+  import CacheSSM
+  import CacheIfc
+  import DiskIfc
+
+  predicate IsReading(machine: CacheSSM.M, addr: nat)
+  {
+    && machine.M?
+    && addr in machine.disk_idx_to_cache_idx
+    && machine.disk_idx_to_cache_idx[addr].Some?
+    && machine.disk_idx_to_cache_idx[addr].value in machine.entries
+    && machine.entries[machine.disk_idx_to_cache_idx[addr].value].Reading?
+  }
+
+  predicate IsWriting(machine: CacheSSM.M, addr: nat)
+  {
+    && machine.M?
+    && addr in machine.disk_idx_to_cache_idx
+    && machine.disk_idx_to_cache_idx[addr].Some?
+    && machine.disk_idx_to_cache_idx[addr].value in machine.statuses
+    && machine.statuses[machine.disk_idx_to_cache_idx[addr].value].Writeback?
+  }
+
+  predicate InverseMapConsistent(machine: CacheSSM.M, i: nat)
+  {
+    && machine.M?
+    && i in machine.disk_idx_to_cache_idx ==>
+      && machine.disk_idx_to_cache_idx[i].Some? ==>
+        && machine.disk_idx_to_cache_idx[i].value in machine.entries
+        && (machine.entries[machine.disk_idx_to_cache_idx[i].value].Reading?
+          || machine.entries[machine.disk_idx_to_cache_idx[i].value].Entry?)
+        && machine.entries[machine.disk_idx_to_cache_idx[i].value].disk_idx == i
+  }
+
+  predicate Inv(s: A.Variables) {
+    && s.machine.M?
+    && (forall i :: i in s.machine.statuses <==>
+        (i in s.machine.entries && s.machine.entries[i].Entry?))
+    && (forall i | i in s.machine.entries ::
+        (s.machine.entries[i].Entry? || s.machine.entries[i].Reading?) ==>
+            s.machine.entries[i].disk_idx in s.machine.disk_idx_to_cache_idx &&
+            s.machine.disk_idx_to_cache_idx[s.machine.entries[i].disk_idx] == Some(i))
+
+    && (forall i :: InverseMapConsistent(s.machine, i))
+
+    && s.machine.read_reqs !! s.machine.read_resps.Keys
+    && (forall rid1, rid2 | rid1 in s.disk.reqReads && rid2 in s.disk.respReads ::
+          s.disk.reqReads[rid1].addr != s.disk.respReads[rid2].addr)
+    && (forall rid1 | rid1 in s.disk.reqReads :: s.disk.reqReads[rid1].addr !in s.machine.read_reqs)
+    && (forall rid1 | rid1 in s.disk.reqReads :: s.disk.reqReads[rid1].addr !in s.machine.read_resps)
+    && (forall rid2 | rid2 in s.disk.respReads :: s.disk.respReads[rid2].addr !in s.machine.read_reqs)
+    && (forall rid2 | rid2 in s.disk.respReads :: s.disk.respReads[rid2].addr !in s.machine.read_resps)
+    && (forall rid1 | rid1 in s.disk.reqReads :: IsReading(s.machine, s.disk.reqReads[rid1].addr))
+    && (forall rid2 | rid2 in s.disk.respReads :: IsReading(s.machine, s.disk.respReads[rid2].addr))
+    && (forall addr | addr in s.machine.read_reqs :: IsReading(s.machine, addr))
+    && (forall addr | addr in s.machine.read_resps :: IsReading(s.machine, addr))
+
+    && s.machine.write_reqs.Keys !! s.machine.write_resps
+    && (forall rid1, rid2 | rid1 in s.disk.reqWrites && rid2 in s.disk.respWrites ::
+          s.disk.reqWrites[rid1].addr != s.disk.respWrites[rid2].addr)
+    && (forall rid1 | rid1 in s.disk.reqWrites :: s.disk.reqWrites[rid1].addr !in s.machine.write_reqs)
+    && (forall rid1 | rid1 in s.disk.reqWrites :: s.disk.reqWrites[rid1].addr !in s.machine.write_resps)
+    && (forall rid2 | rid2 in s.disk.respWrites :: s.disk.respWrites[rid2].addr !in s.machine.write_reqs)
+    && (forall rid2 | rid2 in s.disk.respWrites :: s.disk.respWrites[rid2].addr !in s.machine.write_resps)
+    && (forall rid1 | rid1 in s.disk.reqWrites :: IsWriting(s.machine, s.disk.reqWrites[rid1].addr))
+    && (forall rid2 | rid2 in s.disk.respWrites :: IsWriting(s.machine, s.disk.respWrites[rid2].addr))
+    && (forall addr | addr in s.machine.write_reqs :: IsWriting(s.machine, addr))
+    && (forall addr | addr in s.machine.write_resps :: IsWriting(s.machine, addr))
+  }
+
+  lemma InitImpliesInv(s: A.Variables)
+  //requires A.Init(s)
+  ensures Inv(s)
+  {
+  }
+
+  lemma Start_PreservesInv(s: A.Variables, s': A.Variables, rid: RequestId, input: CacheIfc.Input)
+  requires Inv(s)
+  requires A.NewTicket(s, s', rid, input)
+  ensures Inv(s')
+  {
+    assert s'.machine.entries == s.machine.entries;
+    assert s'.machine.statuses == s.machine.statuses;
+    assert s'.machine.read_reqs == s.machine.read_reqs;
+    assert s'.machine.read_resps == s.machine.read_resps;
+    assert s'.machine.write_reqs == s.machine.write_reqs;
+    assert s'.machine.write_resps == s.machine.write_resps;
+
+    assert forall i :: InverseMapConsistent(s.machine, i) ==> InverseMapConsistent(s'.machine, i);
+    assert forall i :: IsReading(s.machine, i) ==> IsReading(s'.machine, i);
+    assert forall i :: IsWriting(s.machine, i) ==> IsWriting(s'.machine, i);
+  }
+
+  lemma End_PreservesInv(s: A.Variables, s': A.Variables, rid: RequestId, output: CacheIfc.Output)
+  requires Inv(s)
+  requires A.ConsumeStub(s, s', rid, output)
+  ensures Inv(s')
+  {
+    assert s'.machine.entries == s.machine.entries;
+    assert s'.machine.statuses == s.machine.statuses;
+
+    assert forall i :: InverseMapConsistent(s.machine, i) ==> InverseMapConsistent(s'.machine, i);
+    assert forall i :: IsReading(s.machine, i) ==> IsReading(s'.machine, i);
+    assert forall i :: IsWriting(s.machine, i) ==> IsWriting(s'.machine, i);
+  }
+
+  lemma StartRead_PreservesInv(s: A.Variables, s': A.Variables, cache_idx: nat, disk_idx: nat)
+  requires Inv(s)
+  requires CacheSSM.StartRead(s.machine, s'.machine, cache_idx, disk_idx)
+  requires s'.disk == s.disk
+  ensures Inv(s')
+
+  lemma FinishRead_PreservesInv(s: A.Variables, s': A.Variables, cache_idx: nat, disk_idx: nat, data: DiskIfc.Block)
+  requires Inv(s)
+  requires CacheSSM.FinishRead(s.machine, s'.machine, cache_idx, disk_idx, data)
+  requires s'.disk == s.disk
+  ensures Inv(s')
+
+  lemma StartWriteback_PreservesInv(s: A.Variables, s': A.Variables, cache_idx: nat, disk_idx: nat, data: DiskIfc.Block)
+  requires Inv(s)
+  requires CacheSSM.StartWriteback(s.machine, s'.machine, cache_idx, disk_idx, data)
+  requires s'.disk == s.disk
+  ensures Inv(s')
+
+  lemma FinishWriteback_PreservesInv(s: A.Variables, s': A.Variables, cache_idx: nat, disk_idx: nat, data: DiskIfc.Block)
+  requires Inv(s)
+  requires CacheSSM.FinishWriteback(s.machine, s'.machine, cache_idx, disk_idx, data)
+  requires s'.disk == s.disk
+  ensures Inv(s')
+
+  lemma Evict_PreservesInv(s: A.Variables, s': A.Variables, cache_idx: nat, disk_idx: nat, data: DiskIfc.Block, cache_idx2_opt: Option<nat>)
+  requires Inv(s)
+  requires CacheSSM.Evict(s.machine, s'.machine, cache_idx, disk_idx, data, cache_idx2_opt)
+  requires s'.disk == s.disk
+  ensures Inv(s')
+
+  lemma ObserveCleanForSync_PreservesInv(s: A.Variables, s': A.Variables, cache_idx: nat, disk_idx: nat, data: DiskIfc.Block, rid: RequestId, se: set<nat>)
+  requires Inv(s)
+  requires CacheSSM.ObserveCleanForSync(s.machine, s'.machine, cache_idx, disk_idx, data, rid, se)
+  requires s'.disk == s.disk
+  ensures Inv(s')
+
+  lemma ApplyRead_PreservesInv(s: A.Variables, s': A.Variables, cache_idx: nat, disk_idx: nat, data: DiskIfc.Block, rid: RequestId)
+  requires Inv(s)
+  requires CacheSSM.ApplyRead(s.machine, s'.machine, cache_idx, disk_idx, data, rid)
+  requires s'.disk == s.disk
+  ensures Inv(s')
+
+  lemma ApplyWrite_PreservesInv(s: A.Variables, s': A.Variables, cache_idx: nat, disk_idx: nat, data: DiskIfc.Block, new_data: DiskIfc.Block, rid: RequestId)
+  requires Inv(s)
+  requires CacheSSM.ApplyWrite(s.machine, s'.machine, cache_idx, disk_idx, data, new_data, rid)
+  requires s'.disk == s.disk
+  ensures Inv(s')
+
+  lemma MarkDirty_PreservesInv(s: A.Variables, s': A.Variables, cache_idx: nat)
+  requires Inv(s)
+  requires CacheSSM.MarkDirty(s.machine, s'.machine, cache_idx)
+  requires s'.disk == s.disk
+  ensures Inv(s')
+
+  lemma Internal_PreservesInv(s: A.Variables, s': A.Variables)
+  requires Inv(s)
+  requires A.Machine(s, s')
+  ensures Inv(s')
+  {
+    var step :| CacheSSM.InternalStep(s.machine, s'.machine, step);
+    match step {
+      case StartReadStep(cache_idx, disk_idx) =>
+        StartRead_PreservesInv(s, s', cache_idx, disk_idx);
+
+      case FinishReadStep(cache_idx, disk_idx, data) => 
+        FinishRead_PreservesInv(s, s', cache_idx, disk_idx, data);
+
+      case StartWritebackStep(cache_idx, disk_idx, data) =>
+        StartWriteback_PreservesInv(s, s', cache_idx, disk_idx, data);
+
+      case FinishWritebackStep(cache_idx, disk_idx, data) =>
+        FinishWriteback_PreservesInv(s, s', cache_idx, disk_idx, data);
+
+      case EvictStep(cache_idx, disk_idx, data, cache_idx2_opt) =>
+        Evict_PreservesInv(s, s', cache_idx, disk_idx, data, cache_idx2_opt);
+
+      case ObserveCleanForSyncStep(cache_idx, disk_idx, data, rid, se) =>
+        ObserveCleanForSync_PreservesInv(s, s', cache_idx, disk_idx, data, rid, se);
+
+      case ApplyReadStep(cache_idx, disk_idx, data, rid) =>
+        ApplyRead_PreservesInv(s, s', cache_idx, disk_idx, data, rid);
+
+      case ApplyWriteStep(cache_idx, disk_idx, data, new_data, rid) =>
+        ApplyWrite_PreservesInv(s, s', cache_idx, disk_idx, data, new_data, rid);
+
+      case MarkDirtyStep(cache_idx) =>
+        MarkDirty_PreservesInv(s, s', cache_idx);
+    }
+  }
+
+  lemma NextPreservesInv(s: A.Variables, s': A.Variables, op: ifc.Op)
+  //requires Inv(s)
+  //requires A.Next(s, s', op)
+  ensures Inv(s')
+  {
+    match op {
+      case Start(rid, input) => {
+        Start_PreservesInv(s, s', rid, input);
+      }
+      case End(rid, output) => {
+        End_PreservesInv(s, s', rid, output);
+      }
+      case CrashOp => {
+        InitImpliesInv(s');
+      }
+      case InternalOp => {
+        Internal_PreservesInv(s, s');
+      }
+    }
+  }
+
+  function I(s: A.Variables) : B.Variables
+  //requires Inv(s)
+
+  lemma InitRefinesInit(s: A.Variables)
+  //requires A.Init(s)
+  //requires Inv(s)
+  ensures B.Init(I(s))
+  {
+  }
+
+  lemma NextRefinesNext(s: A.Variables, s': A.Variables, op: ifc.Op)
+  //requires Inv(s)
+  //requires Inv(s')
+  //requires A.Next(s, s', op)
+  ensures B.Next(I(s), I(s'), op)
+  {
+  }
+
+}
